first lemma proved

Spring/Ass3/trie.v
@@ -1,5 +1,5 @@
 (* Implement a (binary) trie *)
-Require Import Bool List.
+Require Import Bool List CpdtTactics.
 Set Implicit Arguments.
 
 Section Tries.
@@ -21,6 +21,7 @@ Fixpoint prefix_match (key1 key2: bitstring): bitstring * bitstring :=
     | _, _ => (key1, key2)
   end.
 
+(*
 Fixpoint search (bits: bitstring) (in_trie: trie): option A :=
   match in_trie with
     | Leaf => None
@@ -32,25 +33,20 @@ Fixpoint search (bits: bitstring) (in_trie: trie): option A :=
           | _, _ => None (* Does not match any further *)
        end
   end.
-
-(*
-let rec insert (bits : bool list) (v : 'a) (in_trie : 'a trie) : 'a trie =
-  match in_trie with
-    | Leaf -> Node (Leaf, bits, Some v, Leaf)
-    | Node (ltrie, key, v', rtrie) -> (match prefix_match key bits with
-        | [], [] -> Node (ltrie, key, Some v, rtrie) (*Found, replace val *)
-        | [], true  :: bits' -> Node (ltrie, key, v', (insert bits' v rtrie))
-        | [], false :: bits' -> Node ((insert bits' v ltrie), key, v', rtrie)
-        | _ :: key', true  :: bits' ->
-            let ltrie' = Node (ltrie, key', v', rtrie) in
-            Node (ltrie', [], None, Node (Leaf, bits', Some v, Leaf))
-        | _ :: key', false :: bits' ->
-            let rtrie' = Node (ltrie, key', v', rtrie) in
-            Node (Node (Leaf, bits', Some v, Leaf), [], None, rtrie')
-        | _ :: key', [] -> Node (ltrie, key, Some v, rtrie))
 *)
-
-(* Definition empty_trie {A: Set}: trie A := Leaf. *)
+Fixpoint search (k: bitstring) (t : trie): option A :=
+  match t with
+    | Leaf => None
+    | Node lhs k' v rhs =>
+        match k', k with
+          | nil, nil      => v
+          | nil, b :: k'' => search k'' (if b then rhs else lhs)
+          | _, nil        => None
+          | l :: kl, m :: k'l => 
+              if eqb l m then search k'l (Node lhs kl v rhs) 
+              else None 
+        end
+  end.
 
 
 Fixpoint insert (bits: bitstring) (v: A) (in_trie: trie): trie :=
@@ -70,5 +66,62 @@ Fixpoint insert (bits: bitstring) (v: A) (in_trie: trie): trie :=
           | _ :: key', nil => Node ltrie key (Some v) rtrie
         end
   end.
+
+(* TODO *)
+Lemma search_insert_top :
+  forall (k: bitstring) (v: A) (lhs rhs: trie),
+    search k (Node lhs k (Some v) rhs) = Some v.
+Proof.
+  intro.
+  induction k.
+  + intros.
+    simpl.
+    reflexivity.
+  + intros.
+    simpl.
+    rewrite eqb_reflx.
+    auto.
+Qed.
+
+(* TODO *)
+Lemma search_rec :
+  forall (b: bool) (k k': bitstring) (v: A) (w: option A) (t1 t2: trie),
+    search (b :: k) (insert (b :: k) v (Node t1 (b :: k') w t2)) = 
+    search k (insert k v (Node t1 k' w t2)).
+Proof.
+  intros.
+Admitted.
+
+(* TODO *)
+Lemma correct_even :
+  forall (b: bool) (k k': bitstring) (v: A) (w: option A) (t1 t2: trie),
+    (forall (v: A) (t: trie), search k (insert k v t) = Some v) ->
+      search (b :: k) (insert (b :: k) v (Node t1 (b :: k') w t2)) = Some v.
+Admitted.
+
+Lemma correct_odd:
+  forall (b b': bool) (k k': bitstring) (v: A) (w: option A) (t1 t2: trie),
+    (forall (v: A) (t: trie), search k (insert k v t) = Some v) -> b <> b'
+      -> search (b :: k) (insert (b :: k) v (Node t1 (b' :: k') w t2)) = Some v.
+Admitted.
+    
+
+Theorem insert_then_search:
+  forall (A: Set) (k: bitstring) (v: A) (t: trie A),
+    search k (insert k v t) = Some v.
+  Proof.
+  intros.
+  induction t.
+  
+
+
+    destruct b.
+    destruct b0.
+    reflexivity.
+    destruct b.
+    simpl.
+    reflexivity.
+    induction k.
+    + 
 
 End Tries.
